Axiomatization coming along

SEAR.thy
@@ -1,14 +1,10 @@
 theory SEAR
-imports
-  Pure
-  Soft_Types
+imports FOL_Base
 
 begin
 
 text \<open>
-Shulman's Sets, Elements, And Relations, formulated as a theory of multiply-sorted first-order logic.
-
-The sorts are dependent; to handle this we use Alex Krauss's soft types library.
+Shulman's Sets, Elements, And Relations, formulated as a theory of many-sorted first-order logic.
 \<close>
 
 declare[[eta_contract=false]]
@@ -16,59 +12,135 @@ declare[[eta_contract=false]]
 
 section \<open>Logical foundations\<close>
 
-subsection \<open>The sorts\<close>
+subsection \<open>Meta\<close>
 
-typedecl tx \<comment>\<open>term expressions of the language\<close>
+text \<open>For meta-level nondependent typing: terms are divided into three meta-types.\<close>
 
-type_synonym sort = "tx type"
+class Sort
 
-notation has_type (infix ":" 40)
+typedecl set
+instance set :: Sort ..
+
+typedecl elem
+instance elem :: Sort ..
+
+typedecl rel
+instance rel :: Sort ..
+
+text \<open>
+For object-level dependent typing: the dependent sorts are the sort of elements for each set X, and the relations for each pair of sets A, B.
+Instead of formalizing the sorts directly, we encode sort information in the form of a sort typing judgment @{text ":"}, defined separately for elements and relations.
+\<close>
 
 axiomatization
-  Set  :: sort and
-  Elem :: "tx \<Rightarrow> sort" and
-  Rel  :: "[tx, tx] \<Rightarrow> sort"
+  elem_sorted :: "[elem, set] \<Rightarrow> o" (infix ":" 40) and
+  rel_sorted :: "[rel, set, set] \<Rightarrow> o" ("(_ : _ \<succ> _)" [41, 0, 41] 40)
 
 
 subsection \<open>Sorted FOL and set theory\<close>
 
-typedecl bool
+subsubsection \<open>Quantifiers\<close>
 
-judgment Trueprop :: "bool \<Rightarrow> prop" ("(_)" 5)
+abbreviation all_elem :: "[set, elem \<Rightarrow> o] \<Rightarrow> o"
+  where "all_elem X P \<equiv> \<forall>x. x: X \<longrightarrow> P x"
 
-axiomatization
-  \<comment>\<open>Basic connectives\<close>
-  conj :: "[bool, bool] \<Rightarrow> bool" (infix "\<and>" 30) and
-  disj :: "[bool, bool] \<Rightarrow> bool" (infix "\<or>" 29) and
-  not  :: "bool \<Rightarrow> bool" ("\<not> _" 59) and
+abbreviation ex_elem :: "[set, elem \<Rightarrow> o] \<Rightarrow> o"
+  where "ex_elem X P \<equiv> \<exists>x. x: X \<and> P x"
 
-  \<comment>\<open>Extra-logical connectives\<close>
-  elem_of :: "[tx, tx] \<Rightarrow> bool" (infix "\<in>" 60) and
-  eq      :: "[tx, tx] \<Rightarrow> bool" (infix "=" 60) and
+abbreviation ex1_elem :: "[set, elem \<Rightarrow> o] \<Rightarrow> o"
+  where "ex1_elem X P \<equiv> \<exists>!x. x: X \<and> P x"
 
-  \<comment>\<open>Quantifiers\<close>
-  forall_set  :: "(tx \<Rightarrow> bool) \<Rightarrow> bool" (binder "\<forall>" [10] 11) and
-  exists_set  :: "(tx \<Rightarrow> bool) \<Rightarrow> bool" (binder "\<exists>" [10] 11) and
-  forall_elem :: "[tx, tx \<Rightarrow> bool] \<Rightarrow> bool" and
-  exists_elem :: "[tx, tx \<Rightarrow> bool] \<Rightarrow> bool" and
-  forall_rel  :: "[tx, tx, tx \<Rightarrow> bool] \<Rightarrow> bool" and
-  exists_rel  :: "[tx, tx, tx \<Rightarrow> bool] \<Rightarrow> bool"
+abbreviation all_rel :: "[set, set, rel \<Rightarrow> o] \<Rightarrow> o"
+  where "all_rel A B P \<equiv> \<forall>\<phi>. \<phi>: A \<succ> B \<longrightarrow> P \<phi>"
+
+abbreviation ex_rel :: "[set, set, rel \<Rightarrow> o] \<Rightarrow> o"
+  where "ex_rel A B P \<equiv> \<exists>\<phi>. \<phi>: A \<succ> B \<and> P \<phi>"
+
+abbreviation ex1_rel :: "[set, set, rel \<Rightarrow> o] \<Rightarrow> o"
+  where "ex1_rel A B P \<equiv> \<exists>!\<phi>. \<phi>: A \<succ> B \<and> P \<phi>"
 
 syntax
-  "_forall_elem" :: "[idt, tx, tx \<Rightarrow> bool] \<Rightarrow> bool" ("(\<forall>_: _./ _)" [0, 0, 10] 11)
-  "_exists_elem" :: "[idt, tx, tx \<Rightarrow> bool] \<Rightarrow> bool" ("(\<exists>_: _./ _)" [0, 0, 10] 11)
-  "_forall_rel"  :: "[idt, tx, tx, tx \<Rightarrow> bool] \<Rightarrow> bool" ("(\<forall>_: _ \<succ> _./ _)" [0, 0, 0, 10] 11)
-  "_exists_rel"  :: "[idt, tx, tx, tx \<Rightarrow> bool] \<Rightarrow> bool" ("(\<exists>_: _ \<succ> _./ _)" [0, 0, 0, 10] 11)
+  "_all_elem" :: "[idt, set, o] \<Rightarrow> o" ("(\<forall>_: _./ _)" [0, 0, 10] 11)
+  "_ex_elem"  :: "[idt, set, o] \<Rightarrow> o" ("(\<exists>_: _./ _)" [0, 0, 10] 11)
+  "_ex1_elem" :: "[idt, set, o] \<Rightarrow> o" ("(\<exists>!_: _./ _)" [0, 0, 10] 11)
+  "_all_rel"  :: "[idt, set, set, o] \<Rightarrow> o" ("(\<forall>_: _ \<succ> _./ _)" [0, 0, 0, 10] 11)
+  "_ex_rel"   :: "[idt, set, set, o] \<Rightarrow> o" ("(\<exists>_: _ \<succ> _./ _)" [0, 0, 0, 10] 11)
+  "_ex1_rel"  :: "[idt, set, set, o] \<Rightarrow> o" ("(\<exists>!_: _ \<succ> _./ _)" [0, 0, 0, 10] 11)
 translations
-  "\<forall>x: X. P" \<rightleftharpoons> "CONST forall_elem X (\<lambda>x. P)"
-  "\<exists>x: X. P" \<rightleftharpoons> "CONST exists_elem X (\<lambda>x. P)"
-  "\<forall>\<phi>: A \<succ> B. P" \<rightleftharpoons> "CONST forall_rel A B (\<lambda>\<phi>. P)"
-  "\<exists>\<phi>: A \<succ> B. P" \<rightleftharpoons> "CONST exists_rel A B (\<lambda>\<phi>. P)"
+  "\<forall>x: X. P"  \<rightleftharpoons> "CONST all_elem X (\<lambda>x. P)"
+  "\<exists>x: X. P"  \<rightleftharpoons> "CONST ex_elem X (\<lambda>x. P)"
+  "\<exists>!x: X. P" \<rightleftharpoons> "CONST ex1_elem X (\<lambda>x. P)"
+  "\<forall>\<phi>: A \<succ> B. P"  \<rightleftharpoons> "CONST all_rel A B (\<lambda>\<phi>. P)"
+  "\<exists>\<phi>: A \<succ> B. P"  \<rightleftharpoons> "CONST ex_rel A B (\<lambda>\<phi>. P)"
+  "\<exists>!\<phi>: A \<succ> B. P" \<rightleftharpoons> "CONST ex1_rel A B (\<lambda>\<phi>. P)"
+
+subsubsection \<open>Basic judgments\<close>
+
+axiomatization
+  elem_of :: "[elem, set] \<Rightarrow> o" (infix "\<in>" 50) and
+  holds   :: "[rel, elem, elem] \<Rightarrow> o" ("(_'(_, _'))" [100, 0, 0])
+where
+  elem_of_sort: "x \<in> X \<Longrightarrow> x: X" and
+  holds_dom_sort: "\<phi>: A \<succ> B \<Longrightarrow> \<phi>(x, y) \<Longrightarrow> x: A" and
+  holds_codom_sort: "\<phi>: A \<succ> B \<Longrightarrow> \<phi>(x, y) \<Longrightarrow> y: B"
+
+abbreviation "not_elem_of" :: "[elem, set] \<Rightarrow> o" (infix "\<notin>" 50)
+  where "x \<notin> X \<equiv> \<not> x \<in> X"
+
+subsubsection \<open>Definite description\<close>
+
+axiomatization desc :: "('a \<Rightarrow> o) \<Rightarrow> 'a" where
+  desc_def [intro?]: "\<exists>!x. P x \<Longrightarrow> P (desc P)"
+
+syntax "_the" :: "[idt, o] \<Rightarrow> 'a" ("(the _ | _)")
+translations "the x | P" \<rightleftharpoons> "CONST desc (\<lambda>x. P)"
 
 
-prop "\<exists>A. \<forall>R: A \<succ> A. \<not> R = S"
-ML_val {* @{prop "\<exists>A. \<forall>R: A \<succ> A. \<not> R = S"} *}
+section \<open>Axioms\<close>
 
+axiomatization where
+
+  existence: "\<exists>X. \<exists>x: X. x \<in> X" and
+
+  comprehension: "\<exists>!\<phi>: A \<succ> B. \<forall>x: A. \<forall>y: B. \<phi>(x, y) \<longleftrightarrow> P x y"
+
+text \<open>To state the third axiom we first define functions.\<close>
+
+abbreviation is_func :: "[rel, set, set] \<Rightarrow> o" ("(_ : _ \<rightarrow> _)" [41, 0, 41] 40)
+  where "\<phi>: A \<rightarrow> B \<equiv> \<phi>: A \<succ> B \<and> (\<forall>x. x \<in> A \<longrightarrow> (\<exists>!y. \<phi>(x, y)))"
+
+abbreviation func_app :: "[rel, elem] \<Rightarrow> elem" ("(_'(_'))" [100, 0])
+  where "\<phi>(x) \<equiv> the y | \<phi>(x, y)"
+
+lemma "\<lbrakk>\<phi>: A \<rightarrow> B; x \<in> A\<rbrakk> \<Longrightarrow> \<phi>(x, \<phi>(x))"
+  by rule auto
+
+axiomatization
+  tab :: "rel \<Rightarrow> set" ("|_|") and
+  fst :: "rel \<Rightarrow> rel" and
+  snd :: "rel \<Rightarrow> rel"
+where
+  tabulation:
+    "\<forall>\<phi>: A \<succ> B.
+      fst \<phi>: |\<phi>| \<rightarrow> A \<and>
+      snd \<phi>: |\<phi>| \<rightarrow> B \<and>
+      (\<forall>x: A. \<forall>y: B. \<phi>(x, y) \<longleftrightarrow> (\<exists>r: |\<phi>|. (fst \<phi>)(r) = x \<and> (snd \<phi>)(r) = y)) \<and>
+      (\<forall>r: |\<phi>|. \<forall>s: |\<phi>|. (fst \<phi>)(r) = (fst \<phi>)(s) \<and> (snd \<phi>)(r) = (snd \<phi>)(s) \<longrightarrow> r = s)"
+
+
+subsection \<open>Basic consequences of the axioms\<close>
+
+theorem emptyset: "\<exists>X. \<forall>x: X. x \<notin> X"
+proof -
+  from existence
+    obtain a A where "a \<in> A" by auto
+  from comprehension[of A A "\<lambda>_ _. False"]
+    obtain \<phi> where
+    "\<phi>: A \<succ> A" and
+    "\<forall>x: A. \<forall>y: A. \<not>\<phi>(x, y)"
+    by auto
+  with tabulation[of A A]
+    have 
 
 
 end
