SEAR_old.thy
@@ -1,0 +1,107 @@
+theory SEAR_old
+imports FOL_Base
+
+begin
+
+text \<open>
+Shulman's Sets, Elements, And Relations, formulated as a theory of many-sorted first-order logic.
+\<close>
+
+declare[[eta_contract=false]]
+
+
+section \<open>Logical foundations\<close>
+
+subsection \<open>The sorts\<close>
+
+typedecl t \<comment>\<open>terms of the language\<close>
+instance t :: expr ..
+
+typedecl sort
+instance sort :: expr ..
+
+axiomatization
+  has_type :: "[t, sort] \<Rightarrow> o" (infix ":" 40)
+
+axiomatization
+  Set  :: sort and
+  Elem :: "t \<Rightarrow> sort" and
+  Rel  :: "[t, t] \<Rightarrow> sort"
+
+
+subsection \<open>Sorted FOL and set theory\<close>
+
+no_notation
+  All (binder "\<forall>" 10) and
+  Ex  (binder "\<exists>" 10) and
+  Ex1 (binder "\<exists>!" 10)
+notation
+  All (binder "ALL " 10) and
+  Ex  (binder "EX " 10) and
+  Ex1 (binder "EX! " 10)
+
+text \<open>Quantifiers:\<close>
+
+definition forall_set :: "(t \<Rightarrow> o) \<Rightarrow> o" (binder "\<forall>" [10] 11)
+  where "\<forall>X. P X \<equiv> ALL X. (X: Set \<longrightarrow> P X)"
+
+definition exists_set :: "(t \<Rightarrow> o) \<Rightarrow> o" (binder "\<exists>" [10] 11)
+  where "\<exists>X. P X \<equiv> EX X. (X: Set \<and> P X)"
+
+definition exists1_set :: "(t \<Rightarrow> o) \<Rightarrow> o" (binder "\<exists>!" [10] 11)
+  where "\<exists>!X. P X \<equiv> EX! X. (X: Set \<and> P X)"
+
+definition forall_elem :: "[t, t \<Rightarrow> o] \<Rightarrow> o"
+  where "forall_elem X P \<equiv> ALL x. (x: Elem X \<longrightarrow> P x)"
+
+definition exists_elem :: "[t, t \<Rightarrow> o] \<Rightarrow> o"
+  where "exists_elem X P \<equiv> EX x. (x: Elem X \<and> P x)"
+
+definition exists1_elem :: "[t, t \<Rightarrow> o] \<Rightarrow> o"
+  where "exists1_elem X P \<equiv> EX! x. (x: Elem X \<and> P x)"
+
+definition forall_rel :: "[t, t, t \<Rightarrow> o] \<Rightarrow> o"
+  where "forall_rel A B P \<equiv> ALL \<phi>. (\<phi>: Rel A B \<longrightarrow> P \<phi>)"
+
+definition exists_rel :: "[t, t, t \<Rightarrow> o] \<Rightarrow> o"
+  where "exists_rel A B P \<equiv> EX \<phi>. (\<phi>: Rel A B \<and> P \<phi>)"
+
+definition exists1_rel :: "[t, t, t \<Rightarrow> o] \<Rightarrow> o"
+  where "exists1_rel A B P \<equiv> EX! \<phi>. (\<phi>: Rel A B \<and> P \<phi>)"
+
+syntax
+  "_forall_elem" :: "[idt, t, t \<Rightarrow> o] \<Rightarrow> o" ("(\<forall>_: _./ _)" [0, 0, 10] 11)
+  "_exists_elem" :: "[idt, t, t \<Rightarrow> o] \<Rightarrow> o" ("(\<exists>_: _./ _)" [0, 0, 10] 11)
+  "_exists1_elem" :: "[idt, t, t \<Rightarrow> o] \<Rightarrow> o" ("(\<exists>!_: _./ _)" [0, 0, 10] 11)
+  "_forall_rel"  :: "[idt, t, t, t \<Rightarrow> o] \<Rightarrow> o" ("(\<forall>_: _ \<succ> _./ _)" [0, 0, 0, 10] 11)
+  "_exists_rel"  :: "[idt, t, t, t \<Rightarrow> o] \<Rightarrow> o" ("(\<exists>_: _ \<succ> _./ _)" [0, 0, 0, 10] 11)
+  "_exists1_rel"  :: "[idt, t, t, t \<Rightarrow> o] \<Rightarrow> o" ("(\<exists>!_: _ \<succ> _./ _)" [0, 0, 0, 10] 11)
+translations
+  "\<forall>x: X. P" \<rightleftharpoons> "CONST forall_elem X (\<lambda>x. P)"
+  "\<exists>x: X. P" \<rightleftharpoons> "CONST exists_elem X (\<lambda>x. P)"
+  "\<exists>!x: X. P" \<rightleftharpoons> "CONST exists1_elem X (\<lambda>x. P)"
+  "\<forall>\<phi>: A \<succ> B. P" \<rightleftharpoons> "CONST forall_rel A B (\<lambda>\<phi>. P)"
+  "\<exists>\<phi>: A \<succ> B. P" \<rightleftharpoons> "CONST exists_rel A B (\<lambda>\<phi>. P)"
+  "\<exists>!\<phi>: A \<succ> B. P" \<rightleftharpoons> "CONST exists1_rel A B (\<lambda>\<phi>. P)"
+
+text \<open>Basic formula constructors:\<close>
+
+axiomatization
+  elem_of :: "[t, t] \<Rightarrow> o" (infix "\<in>" 50) and
+  holds   :: "[t, t, t] \<Rightarrow> o" ("(_'(_, _'))" [100, 0, 0])
+
+section \<open>Axioms\<close>
+
+axiomatization where
+  existence: "\<exists>X. \<exists>x: X. x \<in> X" and
+  comprehension: "A: Set \<Longrightarrow> B: Set \<Longrightarrow> \<exists>!\<phi>: A \<succ> B. \<phi>(x, y) \<longleftrightarrow> P x y"
+
+thm exists1_rel_def
+
+theorem
+  assumes "A: Set" "B: Set"
+  shows "\<exists>! \<phi> : A \<succ> B. \<phi>(x, y) \<longleftrightarrow> P x y"
+proof (auto simp: exists1_rel_def ex1_def)
+  obtain \<phi> where "\<phi>: Rel A B" using comprehension[OF assms] ex1_def by 
+
+end
